add isort to demo

demo.v
@@ -104,6 +104,89 @@ Qed.
 (* Beweisbares Sortieren *)
 (* ********************* *)
 
+Require Import List.
+
+Inductive sorted : list nat -> Prop :=
+  | sorted0 : sorted nil
+  | sorted1 : forall n:nat, sorted (n :: nil)
+  | sorted2 : forall (n1 n2:nat) (l: list nat), n1 <= n2 -> 
+              sorted (n2 :: l ) -> sorted (n1 :: n2 :: l).
+
+Hint Resolve sorted0 sorted1 sorted2 : sort.
+
+Theorem sorted_red: forall (n:nat) (l: list nat), sorted(n::l) -> sorted l.
+Proof.
+ intros n l H.
+ inversion H. apply sorted0. assumption.
+Qed.
+
+Fixpoint merge (l1 l2: list nat) : list nat :=
+  match l1, l2 with
+  | _, nil => l1
+  | nil, _ => l2
+  | h1::r1, h2::r2 => if Nat.leb h1 h2 then h1::h2::(merge r1 r2) 
+                                       else h2::h1::(merge r1 r2)
+  end.
+
+Fixpoint split (l : list nat) : (list nat)*(list nat) :=
+  match l with
+  | nil => (nil, nil)
+  | h::nil => (l, nil)
+  | h1::h2::r => match (split r) with
+                 | (l1, l2) => (h1::l1, h2::l2)
+                 end
+  end.
+
+Eval compute in (split (1::2::3::4::5::nil)).
+
+Search({ _ <= _}+{ _ > _}).
+
+Fixpoint insert (n: nat) (l: list nat) : list nat :=
+ match l with
+ | nil => n::nil
+ | h::r => match (Compare_dec.le_gt_dec n h) with
+           | left _ => n::h::r
+           | right _ => h::(insert n r)
+           end
+ end.
 
 
+Lemma insert_sorted: forall (n: nat) (l: list nat),
+ sorted l -> sorted (insert n l).
+Proof.
+ intros n l H.
+ elim H.
+  simpl; auto with sort arith. 
+  intro n0. simpl.
+   case (Compare_dec.le_gt_dec n n0). intros; auto with sort arith.
+   intros. apply sorted2. auto with arith. apply sorted1.
+  intros n1 n2. simpl. 
+   case (Compare_dec.le_gt_dec n n2). intros; auto with sort arith.
+   case (Compare_dec.le_gt_dec n n1). intros; auto with sort arith.
+    intros. auto with sort arith.
+  intros. simpl. 
+   case (Compare_dec.le_gt_dec n n1). intros; auto with sort arith.
+   intros. apply sorted2; assumption.
+Qed.
+
+
+Fixpoint isort (l: list nat) : list nat :=
+ match l with
+ | nil => nil
+ | h::r => insert h (isort r)
+ end.
+
+
+Eval compute in (isort (4::1::5::3::2::nil)).
+
+Theorem isort_sorted: forall (l: list nat), sorted (isort l).
+Proof.
+ intro l.
+ induction l.
+  auto with sort.
+  simpl.
+  apply insert_sorted.
+  assumption.
+  Show Proof.
+Qed.
 
